Auto/Translation/Lam2TH0.lean
@@ -7,11 +7,13 @@ open Lean Embedding.Lam Lam2TH0
 def lam2TH0 (lamVarTy : Array LamSort) (lamEVarTy : Array LamSort) (facts : Array LamTerm) : CoreM String := do
   let (typeHs, termHs, etomHs) ← LamReif.collectLamTermsAtoms lamVarTy lamEVarTy facts
   let bvHs := LamReif.collectLamTermsBitvecs facts
+  let icHs := LamReif.collectLamTermsIntConsts facts
   let sorts :=
     ["thf(sortdecl_int, type, s_int: $tType)."] ++
     bvHs.toList.map (fun l => s!"thf(sortdecl_bv{l.length}, type, s_bv{l.length}: $tType).") ++ 
     typeHs.toList.map (fun i => s!"thf(sortdecl_{i}, type, s_a{i}: $tType).")
   let types :=
+    icHs.toList.map (fun ic => s!"thf(typedecl_icst_{transIntConst ic}, type, {transIntConst ic}: {transIntConstSort ic}).") ++
     bvHs.toList.map (fun l => s!"thf(typedecl_bv{transBitvec l}, type, t_bv{transBitvec l}: s_bv{l.length}).") ++
     (← termHs.toList.mapM (fun i => do
       let .some s := lamVarTy.get? i
