Examples/LeanSMTInt.lean
@@ -5,19 +5,25 @@ These are examples borrowed from the SMT Lean tests,
 import Mathlib.Data.Real.Basic
 import Auto.Tactic
 
--- Arith
+set_option auto.smt true
+set_option trace.auto.smt.printCommands true
+set_option trace.auto.smt.result true
+set_option trace.auto.lamReif.printResult true
 
+-- Arith
 example (n m : Int) (h : 0 < m) : n % m < m := by
-  --smt [h]
-  sorry
+  auto
 
 example (n m k l : Int) : (n - m) * k + l = n*k - m*k + l := by
-  --smt
-  sorry
+  auto
+
+example (n m k l : Int) (hN : n ≥ m) (hK : k ≥ l) : n + k ≥ m + l := by
+  --smt [hN, hK]
+  auto
 
 example (n m k l : Int) (hN : n ≤ m) (hK : k ≤ l) : n + k ≤ m + l := by
   --smt [hN, hK]
-  sorry
+  auto
 
 -- Cong
 
@@ -30,7 +36,7 @@ def MyInt := Int
 def MyInt.add (a b : MyInt) : MyInt := Int.add a b
 
 example (a b : MyInt) : a.add b = b.add a := by
-  sorry
+  auto u[MyInt] d[MyInt.add]
 
 -- Dvd
 
@@ -44,29 +50,12 @@ example
     (h3 : dvd c d)
     (h4 : dvd d e) :
   dvd a e := by
-    have h5 : dvd a c := by
-      -- smt [h1, h2, dvdax]
-      exact dvdax _ _ _ h1 h2
-    have h6 : dvd c e := by
-      -- smt [h3, h4, dvdax]
-      exact dvdax _ _ _ h3 h4
-    -- smt [h5, h6, dvdax]
-    exact dvdax _ _ _ h5 h6
+    auto
 
 -- ForallExists
 
 theorem forallExists : ∀ x : Nat, ∃ y : Int, x ≤ y := by
-  -- smt
-  intro x
-  apply Exists.intro
-  case w => exact Int.ofNat x
-  case h =>
-    induction x with
-    | zero => decide
-    | succ x _ =>
-        simp only [LE.le, Int.le, HSub.hSub, Sub.sub, Int.sub, Neg.neg,
-                   Int.neg, Int.negOfNat, HAdd.hAdd, Add.add, Int.add]
-        simp only [Int.subNatNat, Nat.sub_self, Int.NonNeg.mk]
+  auto
 
 -- Let
 
@@ -83,7 +72,7 @@ example (h : f 10 = 10) : f 10 = 10 := by
   auto
 
 theorem neg (x : Int) : - -x = x := by
-  sorry
+  auto
 
 
 
